오오, 이러니까 뭔가 자연어 읽는 것 같이 느껴지는걸! - 그리고, 개념의 모든 '맥락'을 '타입'으로서 명세해야 하는군!

src/01-01-Introduction/YCSCS1.Introduction.HistoryOfCompiler.SpeedCoding.fst
@@ -14,7 +14,7 @@ type interpreter_t =
 
 type program_develop_t = | Develop of (choice2 speedcoding_t handwritten_t)
 type program_execution_t = | Execution of (choice2 speedcoding_t handwritten_t)
-type today_program_execution_t = | TodayExecution of (choice2 speedcoding_t handwritten_t)
+type today_program_execution_t = | TodayExecution of (choice2 interpreter_t Base.executable_t)
 
 //---|
 
@@ -23,20 +23,45 @@ private let c_SpeedCoding = 0
 private let c_HandWritten = 1
 //---|
 
-let is_develop_slower_than (pd1 pd2: program_develop_t) : bool =
-  match (encode_choice2 pd1._0), (encode_choice2 pd2._0) with
+private let _sorh_t = (choice2 speedcoding_t handwritten_t)
+
+private let _is_any_slower_than 
+  (#any_t: Type) (#sel_t: Type)
+  (selector: any_t -> sel_t)
+  (strict_comparer: sel_t -> sel_t -> bool)
+  (any1 any2: any_t)
+  : bool =
+  let (sel1, sel2) = (selector any1, selector any2) in
+  strict_comparer sel1 sel2
+
+(*
+private let _first_is_slower (sorh1 sorh2: _sorh_t) : bool =
+  match encode_choice2 sorh1, encode_choice2 sorh2 with
   | c_HandWritten, c_SpeedCoding -> true
   | _ -> false
+
+private let _speedcoding_is_slower sorh1 sorh2 : bool =
+  not (_handwritten_is_slower sorh1 sorh2)
+*)
+
+let is_develop_slower_than (pd1 pd2: program_develop_t) : bool =
+  _is_any_slower_than (fun (pd: program_develop_t) -> encode_choice2 pd._0) (>) pd1 pd2
 
 let is_less_productive_than pd1 pd2 = is_develop_slower_than pd1 pd2
 
 let is_execution_slower_than (pe1 pe2: program_execution_t) : bool =
-  match (encode_choice2 pe1._0), (encode_choice2 pe2._0) with
-  | c_HandWritten, c_SpeedCoding -> true
-  | _ -> false
+  _is_any_slower_than (fun (pe: program_execution_t) -> encode_choice2 pe._0) (<) pe1 pe2
 
 let is_today_execution_slower_than (pe1 pe2: today_program_execution_t) : bool =
-  match (encode_choice2 pe1._0), (encode_choice2 pe2._0) with
-  | c_HandWritten, c_SpeedCoding -> true
-  | _ -> false
+  _is_any_slower_than (fun (pe: today_program_execution_t) -> encode_choice2 pe._0) (<) pe1 pe2
+
+//--- test ---
+private let c12 = Choice1Of2
+private let c22 = Choice2Of2
+
+let _ = assert ( Develop (c22 HandWritten) `is_develop_slower_than` Develop (c12 SpeedCoding) )
+let _ = assert ( Develop (c22 HandWritten) `is_less_productive_than` Develop (c12 SpeedCoding) )
+let _ = assert ( Execution (c12 SpeedCoding) `is_execution_slower_than` Execution (c22 HandWritten) )
+let _ = assert ( TodayExecution (c12 (OtherInterpreter Base.Interpreter)) `is_today_execution_slower_than` TodayExecution (c22 Base.Executable) )
+//---|
 
